Tangle.lean
@@ -24,8 +24,6 @@ theorem tangle_slice_begin_is_tangle (t : Tangle) (i : Nat) : isTangle (Wall.sli
 end Tangle
 
 namespace PlanarIsotopy
-open PlanarIsotopy
-
 theorem verts_domain_eq_n { n : Nat } : Bricks.domain (vert_bricks n) = n := by
   induction n <;> rw [vert_bricks, Bricks.domain, List.map, List.foldr]
   case succ n' h =>
@@ -53,6 +51,7 @@ theorem tangle_invariant : { a b : Wall } → Map a b → (isTangle a = isTangle
 
 end PlanarIsotopy
 
+
 namespace Reidemeister
 theorem tangle_invariant : { a b : Wall } → Move a b → (isTangle a ↔ isTangle b) := by
   intro a b m
@@ -63,128 +62,191 @@ theorem tangle_invariant : { a b : Wall } → Move a b → (isTangle a ↔ isTan
 
 end Reidemeister
 
+structure Graph (α : Type) [BEq α] where
+  V: List α
+  E: List (α × α)
+  deriving Repr
 
-def Brick.threadEquiv : Brick → Nat → Nat → List (Int × Int)
-  | Vert, i, o => [⟨o, -i⟩]
-  | Cup, i, _o => [⟨-i, -(i.succ)⟩]
-  | Cap, _i, o => [⟨o, o.succ⟩]
-  | Over, i, o => [⟨o, -(i.succ)⟩, ⟨o.succ, -i⟩]
-  | Under, i, o => [⟨o, -(i.succ)⟩, ⟨o.succ, -i⟩]
+namespace Graph
+def from_edges {α : Type} [BEq α] (e : List (α × α)) : Graph α :=
+  Graph.mk (e.foldr (fun n ns =>
+      let ns := ite (ns.contains n.fst) ns (n.fst::ns)
+      ite (ns.contains n.snd) ns (n.snd::ns)
+    ) []) e
 
-structure Bricks.threadEquivAcc where
-  i: Nat
-  o: Nat
-  equiv: List (Int × Int)
-def Bricks.threadEquivFold (b : Brick) (acc : Bricks.threadEquivAcc) : Bricks.threadEquivAcc :=
-  Bricks.threadEquivAcc.mk (acc.i + b.domain) (acc.o + b.codomain) (acc.equiv.append (b.threadEquiv acc.i acc.o))
-/-- returns a list of equivalencies between all threads in the domain and codomain
-threads in the domain are counted up from 0, and threads in the codomain are counted down from -1 -/
-def Bricks.threadEquiv (bs : Bricks) : List (Int × Int) :=
-  (List.foldr Bricks.threadEquivFold (Bricks.threadEquivAcc.mk 0 1 []) bs).equiv
+structure Acc where
+  N: Nat
+  I: List Nat
+  O: List Nat
+  E: List (Nat × Nat)
+  deriving Repr
 
-structure Brick.threadEquiv2Acc (ID : Type) where
-  i: List ID
-  o: List ID
-  equiv: List (ID × ID)
-def Brick.threadEquiv2 {ID : Type} (b : Brick) (acc : Brick.threadEquiv2Acc ID) (enough : b.domain ≤ acc.i.length ∧ b.codomain ≤ acc.o.length) : Brick.threadEquiv2Acc ID :=
-  match b, enough with
-    | Vert, h =>
-      let i := acc.i[0]'(And.left h)
-      let o := acc.o[0]'(And.right h)
-      Brick.threadEquiv2Acc.mk (acc.i.drop 1) (acc.o.drop 1) (⟨i, o⟩ :: acc.equiv)
-    | Cup, h =>
-      let i1 := acc.i[0]'(@Nat.lt_trans 0 1 acc.i.length (by simp) (And.left h))
-      let i2 := acc.i[1]'(And.left h)
-      Brick.threadEquiv2Acc.mk (acc.i.drop 2) acc.o (⟨i1, i2⟩ :: acc.equiv)
-    | Cap, h =>
-      let o1 := acc.o[0]'(@Nat.lt_trans 0 1 acc.o.length (by simp) (And.right h))
-      let o2 := acc.o[1]'(And.right h)
-      Brick.threadEquiv2Acc.mk acc.i (acc.o.drop 2) (⟨o1, o2⟩ :: acc.equiv)
-    | Over, h =>
-      let i1 := acc.i[0]'(@Nat.lt_trans 0 1 acc.i.length (by simp) (And.left h))
-      let i2 := acc.i[1]'(And.left h)
-      let o1 := acc.o[0]'(@Nat.lt_trans 0 1 acc.o.length (by simp) (And.right h))
-      let o2 := acc.o[1]'(And.right h)
-      Brick.threadEquiv2Acc.mk (acc.i.drop 2) (acc.o.drop 2) (⟨i1, o2⟩ :: ⟨i2, o1⟩ :: acc.equiv)
-    | Under, h =>
-      let i1 := acc.i[0]'(@Nat.lt_trans 0 1 acc.i.length (by simp) (And.left h))
-      let i2 := acc.i[1]'(And.left h)
-      let o1 := acc.o[0]'(@Nat.lt_trans 0 1 acc.o.length (by simp) (And.right h))
-      let o2 := acc.o[1]'(And.right h)
-      Brick.threadEquiv2Acc.mk (acc.i.drop 2) (acc.o.drop 2) (⟨i1, o2⟩ :: ⟨i2, o1⟩ :: acc.equiv)
-
-theorem Bricks.head_domain_le_domain (bs : Bricks) (b : Brick) : b.domain ≤ Bricks.domain (b::bs) := by
-  cases b
-  <;> rw [Bricks.domain, List.map, List.foldr]
-  <;> apply Nat.le_add_right
-theorem Bricks.head_codomain_le_codomain (bs : Bricks) (b : Brick) : b.codomain ≤ Bricks.codomain (b::bs) := by
-  cases b
-  <;> rw [Bricks.codomain, List.map, List.foldr]
-  <;> apply Nat.le_add_right
-theorem Bricks.tail_domain_le_domain (bs : Bricks) (b : Brick) : bs.domain ≤ Bricks.domain (b::bs) := by
-  cases b
-  <;> rw [Bricks.domain, Bricks.domain, ←Bricks.domain, List.map, List.foldr, ←Bricks.domain]
-  <;> apply Nat.le_add_left
-theorem Bricks.tail_codomain_le_codomain (bs : Bricks) (b : Brick) : bs.codomain ≤ Bricks.codomain (b::bs) := by
-  cases b
-  <;> rw [Bricks.codomain, Bricks.codomain, ←Bricks.codomain, List.map, List.foldr, ←Bricks.codomain]
-  <;> apply Nat.le_add_left
-
-
-theorem Bricks.threadEquiv2_enough_head_enough
-  {ID : Type} {bs : Bricks} {b : Brick} {acc : Brick.threadEquiv2Acc ID}
-  (enough : (Bricks.domain (b::bs)) ≤ acc.i.length ∧ (Bricks.codomain (b::bs)) ≤ acc.o.length)
-  : b.domain ≤ acc.i.length ∧ b.codomain ≤ acc.o.length
-  := And.intro
-    (Nat.le_trans (Bricks.head_domain_le_domain bs b) enough.left)
-    (Nat.le_trans (Bricks.head_codomain_le_codomain bs b) enough.right)
-theorem Bricks.threadEquiv2_preserves_len
-  {ID : Type} (bs : Bricks) (b : Brick) (acc : Brick.threadEquiv2Acc ID) 
-  (enough : (Bricks.domain (b::bs)) ≤ acc.i.length ∧ (Bricks.codomain (b::bs)) ≤ acc.o.length)
-  : bs.domain ≤ (b.threadEquiv2 acc (Bricks.threadEquiv2_enough_head_enough enough)).i.length
-    ∧ bs.codomain ≤ (b.threadEquiv2 acc (Bricks.threadEquiv2_enough_head_enough enough)).o.length :=
-  have add_le_length_le_drop {α : Type} {n m : Nat} {l : List α} (le_plus : m + n ≤ l.length) : n ≤ (l.drop m).length := by
-      sorry
-
-  And.intro
-    (by
-      have enough := enough.left
-      rw [threadEquiv2]
-      have add_le_length : (b.domain) + (domain bs) ≤ acc.i.length := by
-        rw [domain, List.map, List.foldr, ←domain] at enough
+-- specialized List.zip which carries proof that lengths are equal
+def zip_eq (a b : List Nat) (leneq : a.length = b.length) : List (Nat × Nat) := match a, b with
+  | [], [] => []
+  | a::a', b::b' => 
+      have leneq' : a'.length = b'.length := by
+        simp [List.length] at leneq
         assumption
-      cases b <;> simp <;> apply add_le_length_le_drop add_le_length
-    )
-    (by
-      have enough := enough.right
-      rw [threadEquiv2]
-      have add_le_length : (b.codomain) + (codomain bs) ≤ acc.o.length := by
-        rw [codomain, List.map, List.foldr, ←codomain] at enough
-        assumption
-      cases b <;> simp <;> apply add_le_length_le_drop add_le_length
-    )
+      (Prod.mk a b)::(zip_eq a' b' leneq')
+
+def stack (acc acc': Acc) (iolen: acc.O.length = acc'.I.length) : Acc :=
+  Acc.mk
+    (Nat.max acc.N acc'.N)
+    acc.I
+    acc'.O
+    (((zip_eq acc.O acc'.I iolen).append acc.E).append acc'.E)
+
+theorem stack_length_eq {acc acc' : Acc} {iolen : acc.O.length = acc'.I.length} :
+  (stack acc acc' iolen).I.length = acc.I.length ∧ (stack acc acc' iolen).O.length = acc'.O.length := by
+  rewrite [stack]
+  simp
+
+def acc_brick : Brick → Acc → Acc
+  | Vert,  ⟨n, i, o, e⟩ => ⟨n+2, n::i,        (n+1)::o,        ⟨n, n+1⟩::e⟩
+  | Cap,   ⟨n, i, o, e⟩ => ⟨n+2, i,           (n+1)::n::o,     ⟨n, n+1⟩::e⟩
+  | Cup,   ⟨n, i, o, e⟩ => ⟨n+2, (n+1)::n::i, o,               ⟨n, n+1⟩::e⟩
+  | Over,  ⟨n, i, o, e⟩ => ⟨n+4, (n+1)::n::i, (n+3)::(n+2)::o, ⟨n, n+3⟩::⟨n+1, n+2⟩::e⟩
+  | Under, ⟨n, i, o, e⟩ => ⟨n+4, (n+1)::n::i, (n+3)::(n+2)::o, ⟨n, n+3⟩::⟨n+1, n+2⟩::e⟩
+
+def acc_bricks (bs: Bricks) (acc: Acc) : Acc := match bs with
+  | [] => acc
+  | b::bs => acc_brick b (acc_bricks bs acc)
+
+
+theorem acc_brick_io {b : Brick} {acc : Acc} :
+      ((acc_brick b acc).I.length = acc.I.length + b.domain)
+    ∧ ((acc_brick b acc).O.length = acc.O.length + b.codomain) := by
+  cases b <;> simp [acc_brick, Brick.domain, Brick.codomain]
+
+theorem acc_bricks_io {bs : Bricks} {acc : Acc} :
+      ((acc_bricks bs acc).I.length = acc.I.length + bs.domain)
+    ∧ ((acc_bricks bs acc).O.length = acc.O.length + bs.codomain) := by
+  induction bs
+  case nil => simp [acc_bricks, Bricks.domain, Bricks.codomain, List.foldr]
+  case cons hd tl hind =>
+    simp [acc_bricks, List.length, Bricks.domain, Bricks.codomain, List.foldr]
+    rewrite [←Bricks.domain, ←Bricks.codomain]
+    apply And.intro
+    case left =>
+      rewrite [Nat.add_comm hd.domain _, ←Nat.add_assoc]
+      rewrite [acc_brick_io.left, hind.left]
+      rfl
+    case right =>
+      rewrite [Nat.add_comm hd.codomain _, ←Nat.add_assoc]
+      rewrite [acc_brick_io.right, hind.right]
+      rfl
+
+
+def acc_tangle_aux (bs : Bricks) (w : Wall) (ht : isTangle (bs::w)) (acc : Acc) (domeq : bs.domain = acc.O.length) : Acc := match w, ht with
+  | [], _ =>
+      let acc' := acc_bricks bs (Acc.mk acc.N [] [] [])
+      have hs: acc.O.length = acc'.I.length := by
+        rewrite [acc_bricks_io.left, List.length, domeq, Nat.add_comm, Nat.add_zero]
+        exact Eq.refl _
+      stack acc acc' hs
+  | bs'::w, ht =>
+      let acc' := acc_bricks bs (Acc.mk acc.N [] [] [])
+      have hs: acc.O.length = acc'.I.length := by
+        rewrite [acc_bricks_io.left, List.length, domeq, Nat.add_comm, Nat.add_zero]
+        exact Eq.refl _
+      let acc := stack acc acc' hs
+      have hs' : bs'.domain = acc.O.length := by
+        have codomeq : bs.codomain = acc.O.length := by
+          rewrite [stack_length_eq.right, acc_bricks_io.right]
+          simp
+        rw [isTangle] at ht
+        rw [←ht.left]
+        exact codomeq
+      have ht' : isTangle (bs'::w) := by
+        rw [isTangle] at ht
+        exact ht.right
+      acc_tangle_aux bs' w ht' acc hs'
+def acc_tangle : (t: Tangle) → (acc: Acc) → (domeq: t.domain = acc.O.length) → Acc
+  | ⟨[], _⟩, acc, _ => acc
+  | ⟨bs::w, prop⟩, acc, domeq => acc_tangle_aux bs w prop acc domeq
+
+
+#eval [0, 1, 2].partition (fun n => n ≥ 1)
+-- merges inhabited lists
+def reduceAux {α : Type} [BEq α] (v : List (α × List α)) : List (α × α) → List (α × List α)
+  | [] => v
+  | ⟨a, b⟩::e =>
+      let vnew := v.partition (fun vs => (vs.snd.contains a) ∨ (vs.snd.contains b))
+      let vnew := match vnew.fst with
+        | [] => vnew.snd
+        | hd::tl => ⟨hd.fst, (hd::tl).foldr (fun x acc => x.snd.append acc) []⟩::vnew.snd
+      reduceAux vnew e
+def reduce {α : Type} [BEq α] (g : Graph α) : Graph α :=
+  let v' := reduceAux (g.V.map (fun v => ⟨v, [v]⟩)) g.E
+  let v' := v'.map Prod.fst
+  Graph.mk v' []
+
+namespace Example
+def g : Graph Nat := Graph.from_edges [⟨0, 1⟩]
+#eval g
+#eval Graph.reduceAux (g.V.map (fun v => ⟨v, [v]⟩)) g.E
+#eval Graph.reduce g
+end Example
+
+end Graph
+
+
+namespace Nat
+def sequence : Nat → List Nat
+  | 0 => []
+  | n+1 => n::(sequence n)
+
+theorem sequence_length_eq_n {n : Nat} : (sequence n).length = n := by
+  induction n
+  case zero =>
+    rewrite [sequence, List.length]
+    exact Eq.refl _
+  case succ n ind =>
+    rewrite [sequence, List.length, Nat.succ_eq_add_one, ind]
+    exact Eq.refl _
+end Nat
+
 
 namespace Tangle
-theorem bricks_domain_is_monotonic : ∀ b : Brick, ∀ bs : Bricks, b.domain ≤ Bricks.domain (b::bs) := by
-  intro b bs
-  induction bs
-  case nil =>
-    rw [Bricks.domain, List.map, List.map, List.foldr, List.foldr, Nat.add]
-    apply Nat.le_of_eq
-    rfl
-  case cons b' bs' h =>
-    have h' : Bricks.domain (b::bs') ≤ Bricks.domain (b::b'::bs') := by
-      repeat rw [Bricks.domain]
-      repeat rw [List.map]
-      repeat rw [List.foldr]
-      simp
-      rw [←(Nat.add_assoc _ (Brick.domain b') _), Nat.add_comm _ (Brick.domain b'), Nat.add_assoc]
-      apply Nat.le_add_left
-    apply Nat.le_trans h h'
-
-
--- don't know how to calculate this yet
 /-- thread count is to tangle as link number is to links -/
-def threadCount (t : Tangle) : Nat := sorry
+def thread_count (t : Tangle) : Nat :=
+  let acc0 : Graph.Acc := ⟨0, [], Nat.sequence t.domain, []⟩
+  let acc := Graph.acc_tangle t acc0 (Eq.symm Nat.sequence_length_eq_n)
+  let ind_graph := Graph.reduce (Graph.from_edges acc.E)
+  ind_graph.V.length
+
+
+namespace Example
+def ltrefoil : Tangle :=
+  let trefoil : Wall := [
+    [Cap],
+    [Vert, Cap, Vert],
+    [Over, Over],
+    [Vert, Under, Vert],
+    [Cup, Cup]
+  ]
+  ⟨trefoil, by simp [isTangle]⟩
+
+#eval Nat.sequence ltrefoil.domain
+#eval Graph.acc_tangle ltrefoil ⟨0, [], Nat.sequence ltrefoil.domain, []⟩ (Eq.symm Nat.sequence_length_eq_n)
+#eval Graph.reduce (Graph.from_edges [⟨0,1⟩, ⟨1,2⟩, ⟨2,0⟩])
+#eval Graph.reduce (Graph.from_edges (Graph.acc_tangle ltrefoil ⟨0, [], Nat.sequence ltrefoil.domain, []⟩ (Eq.symm Nat.sequence_length_eq_n)).E)
+#eval thread_count ltrefoil
+
+
+def hopf_link : Tangle :=
+  let hopf_link : Wall := [
+    [Cap, Cap],
+    [Vert, Over, Vert],
+    [Vert, Over, Vert],
+    [Cup, Cup]
+  ]
+  ⟨hopf_link, by simp [isTangle]⟩
+
+#eval thread_count hopf_link
+end Example
 
 end Tangle
+
+
