lakefile.lean
@@ -5,15 +5,9 @@ package knot {
   -- add package configuration options here
 }
 
-lean_lib Knot {}
-
 lean_lib Basic {}
 
 lean_lib Tangle {}
 
 lean_lib Link {}
 
---@[defaultTarget]
---lean_exe knot {
---  root := `Main
---}
