lean3/src/link.lean
@@ -1,3 +1,0 @@
-import tangle
-
-def link := { t : tangle // t.domain = 0 ∧ t.codomain = 0 }
